\section{10.5 Edfinity: The Ratio and Root Test}
\begin{itemize}
  \item The ratio test: assume \(\displaystyle \rho = \lim_{n \to \infty}
    \left| \frac{a_{n+1}}{a_n} \right| \) exists, then:
    \begin{itemize}
      \item \(\sum a_n\) converges absolutely if \(\rho < 1\).
      \item \(\sum\) diverges if \(\rho > 1\).
      \item Inconclusive if \(\rho = 1\).
    \end{itemize}
  \item Root test: assume that \(\displaystyle L = \lim_{n \to \infty} \left|
    a_n \right|^{\frac{1}{n}}\) exists, then
    \begin{itemize}
      \item \(\sum a_n\) converges absolutely if \(L < 1\).
      \item \(\sum\) diverges if \(L > 1\).
      \item Inconclusive if \(L = 1\).
    \end{itemize}

  \item[1.] Apply the Ratio test:
  \begin{align*}
    \sum_{n=1}^{\infty} 6^{-n}\\
    a_{n+1} = 6^{-n-1}, \quad a_n = 6^{-1} \\
    \then \rho = \lim_{n \to \infty} \left|  6^{-n-1}  \cdot 6^{n} \right| = 6^{-1}
  \end{align*}

  \item[2.] Apply the Ratio test:
  \begin{align*}
    \sum_{n=1}^{\infty} \frac{1}{n\ln n} \\
    &\then \rho = \lim_{n \to \infty}
    \left| \frac{n \ln  n}{(n+1) \ln (n+1)} \right| \\
    &\then \lim_{n \to \infty} \frac{\ln n + 1}{\ln (n+1)+1} \\
    &\then \lim_{i \to \infty} \frac{n}{n+1} \\
    &\then \lim_{n \to \infty} = 1
  \end{align*}

  \item[3.] Apply the Ratio test:
    \begin{align*}
      \sum_{n=1}^{\infty} \left|\frac{(-5)^k}{k!} \right| \\
      \lim_{n \to \infty} = \frac{(5)^k+1}{(k+1)k!} \cdot \frac{k!}{(5)^k} =
      \frac{5}{k+1} = 0
    \end{align*}

  \newpage

  \item[4.] Apply the Root test:
    \begin{align*}
      \sum_{n=1}^{\infty} n^{-8n} \\
      &\then \lim_{n \to \infty} (n^{-8n})^{n^{-1}} \\
      &\then \lim_{n \to \infty} n^{-8} = 0
    \end{align*}

  \item[5.] Apply the Root test:
    \begin{align*}
      \sum_{n=1}^{\infty} \left( \frac{n+9}{3n+14} \right)^n \\
      \then \lim_{n \to \infty}\frac{n+9}{3n+14} = \frac{1}{3}
    \end{align*}


  \item[6.] Apply the Root test:
    \begin{align*}
      \sum_{n=1}^{\infty} \left(1+(5n)^{-1}\right)^{-n^2}\\
      \then \lim_{n \to \infty} \left|  \left(1+(5n)^{-1}\right)^{-n^2} \right|^{n^{-1}}  \\
      \then  \lim_{n \to \infty} \left(1+(5n)^{-1}\right)^{-n} = e^{-\frac{1}{5}}
    \end{align*}

  \item Determine convergence:
    \begin{align*}
      \sum_{n=1}^{\infty} \frac{n^2+9n+6}{9n^4 + 4n^3 + 4n^2 + 4} \\
      a_n = \frac{n^2+9n+6}{9n^4 + 4n^3 + 4n^2 + 4}, \quad b_n = \frac{n^2+9n+6}{9n^4} \\
      \then \lim_{n \to \infty}\frac{n^2+9n+6}{9n^4 + 4n^3 + 4n^2 + 4} \cdot \frac{9n^4}{n^2+9n+6} \\
      \then \lim_{n \to \infty} \frac{1}{4n^3+4n^2+4} =0 \\
    \end{align*}

  \item Determine convergence:
    \begin{align*}
      \sum_{n=1}^{\infty} \sin \left( n^{-2} \right) \\
      a_n = \sin (n^{-2}), \quad b_n = n^{-2} \\
      \sin n^{-2} \leq n^{-2} \\
      \sum_{n=1}^{\infty}\sin n^{-2} \leq  \sum_{n=i}^{\infty}n^{-2} \\
      b_n ~\text{converges by p-series}~\\
      \then a_n ~\text{converges}~
    \end{align*}

  \item Determine convergence:
    \begin{align*}
      \sum_{n=1}^{\infty} \left( \frac{n}{n+13} \right) ^n \\
      &\then \lim_{n \to \infty} \left( \frac{n}{n+13} \right)^n = e^{-13}
    \end{align*}

\end{itemize}
