% chktex-file 1
% chktex-file 3
% chktex-file 21
% chktex-file 36
% chktex-file 27

\chapter{Introduction to Differential Equations}
\section{9.1 Edfinity: Solving Differential Equations}
\begin{itemize}
  \item[]

  \subsection{9.1.5}
  \begin{itemize}
    \item Solve \( y' = x^5y^2 \), using separation of variables, given the
      initial condition \( y\left( 0 \right) = 9   \)
      \begin{align*}
        \frac{\frac{dy}{dx}}{y^2} &= x^5\\
        \int \frac{\frac{dy}{dx}}{y(x)^2} &= \int x^5 dx \\
        -\frac{1}{y(x)} &= \frac{x^6}{6} + c_1 \\
        y(x) &= -\frac{6}{x^6 + c_1} \\
        9 &= - \frac{6}{c}, \quad c = -\frac{6}{9} \\
        \Aboxed{y(x) &= - \frac{18}{2x^6 - 2}}
      \end{align*}
  \end{itemize}

  \subsection{9.1.6}
  \begin{itemize}
    \item Solve the initial value problem \( \frac{dy}{dx} + 3y = 0,\quad y(\ln 4) =
      3 \).
    \begin{align*}
      \frac{dy}{dx} &= -3y \\
      \int \frac{dy}{dx} y^{-1}dx &= \int -3dx \\
      \ln|y| &= -3x + \lambda \\
      y &= e^{-3x} \lambda \\
      3 &= e^{3(\ln 4)} \lambda \then \lambda = 192 \\
      y &= 192e^{-3x}
    \end{align*}

  \end{itemize}

  \subsection{9.1.7}
  \begin{itemize}
    \item Solve \( (t^2 + 36)\frac{dx}{dt} = (x^2+9) \), using separation of
      variables, given the initial condition \( x(0)=3 \).
      \begin{align*}
        \frac{dx}{dt} &= \left( t^2+36 \right)^{-1} \\
        \frac{dx}{dt} \left( x^2 + 9 \right)^{-1} &= (t^2 + 36)^{-1} \\
        \int\frac{dx}{dt} \left( x^2 + 9 \right)^{-1} &= \int (t^2 + 36)^{-1}dt \\
        \frac{1}{9}\int \left(\frac{x^2}{9}+1\right)^{-1}dx &= \frac{1}{36} \int \left(\frac{t^2}{36} + 1\right)^{-1} dt \\
        \frac{1}{3}\tan ^{-1}\left( \frac{x}{3} \right) &= \frac{1}{6} \tan ^{-1} \left( \frac{t}{6} \right) + \lambda \\
        \tan ^{-1} \left( \frac{x}{3} \right) &= \frac{1}{2}\tan ^{-1}\left( \frac{t}{6} \right) + \lambda \\
        \tan ^{-1} \left( \frac{3}{3} \right) &= \frac{1}{2}\tan ^{-1}\left( \frac{0}{6} \right) + \lambda \\
        \frac{\pi}{4} &= \lambda \\
        x &= 3\tan \left( \frac{1}{2}\tan ^{-1}\left( \frac{t}{6} \right) + \frac{\pi}{4} \right)
      \end{align*}
  \end{itemize}

  \subsection{9.1.8}
  \begin{itemize}
    \item Solve the initial value problem \( \frac{dy}{dx} = \left( x-7 \right) (y-8), \quad y\left( 0 \right) = 4 \)
      \begin{align*}
        \frac{dy}{dx} \left( y-8 \right) ^{-1} &= \left( x-7 \right) \\
        \int dy \left( y-8 \right) ^{-1} &= \int \left( x-7 \right) dx\\
        \ln y-8 &= x^{-2} -7x + \lambda \\
        y &= e^{\frac{x^2}{2}-7x}\lambda + 8 \\
        -4 &= \lambda \\
        y &= -4e^{\frac{x^2}{2}-7x} + 8
      \end{align*}
  \end{itemize}

  \subsection{9.1.9}
  \begin{itemize}
    \item Solve the initial value problem \( t^2 \frac{dy}{dt} - t = 1 + y +
      ty, \quad y(1) = 7 \)
      \begin{align*}
        \int\left( y + 1 \right) dy &= \int\frac{1+t}{t^2}dt \\
        \ln |1+y| &= -t^{-1}+\ln t + \lambda \\
        y &= \lambda e^{-t^{-1} + \ln t} - 1 = \lambda \frac{t}{e^{t^{-1}}} - 1\\
        7 &= \lambda e^{-1} - 1 \\
        \lambda &= 8e \\
        y &= 8te^{1-t^{-1}} - 1
      \end{align*}
  \end{itemize}

  \subsection{9.1.10}
  \begin{itemize}
    \item Solve the initial value problem \( y' = 2y^2 \sin x, \quad y(0)=6 \)
       \begin{align*}
          \frac{dy}{dx}(2y^2)^{-1} &= \sin x \\
          \int \frac{dy}{dx} y^{-2} dx &= \int 2\sin x dx  \\
          -y^{-1} &= -2\cos x + \lambda \\
          y &= (2\cos x + \lambda)^{-1} \\
          6 &= \left( 2\cos 0 + \lambda \right) ^{-1} \\
          -\frac{11}{6} &= \lambda \\
          y &= \left( 2\cos x - \frac{11}{6} \right)^{-1}
       \end{align*}
  \end{itemize}

\end{itemize}
