\section{9.5 Edfinity: First-Order Linear Equations}
\begin{itemize}
  \item Hammers:
    \begin{align*}
      y' + P(x)y &= Q(x)  \\
      \alpha(x) &= e^{\int P(x)dx} \\
      y &= \alpha(x)^{-1}\left(\int \alpha(x)Q(x)dx + C\right)
    \end{align*}

  \subsection{9.5.1}
  \begin{itemize}
    \item Solve \(y' + 3x^{-1}y = x^2, \qquad y(1) = -9\)
      \begin{itemize}
        \item Idetify the integrating factor, \(\alpha(x)\)
          \begin{align*}
            \alpha(x) &= e^{\int 3x^{-1} dx}  \\
            \alpha(x) &= e^{3\ln x} \\
            \alpha(x) &= x^3
          \end{align*}

        \item Find the general solution, \(y(x)\)
          \begin{align*}
            y &= x^{-3}\left(\int x^3x^2 dx + C\right) \\
            y &= x^{-3}\left(\frac{x^{6}}{6} + C\right) \\
            y &= \frac{x^3}{6} + Cx^{-3}
          \end{align*}

        \item Solve the innitla value problem, \(y(1) = - 9\)
          \begin{align*}
            -9 &= \frac{1^3}{6} + C^{-3} \\
            1.5 &= C^{-3} \\
            C &= -\left(\frac{55}{6}\right)^{3^{-1}} \\
            \then
            y &= \frac{x^3}{6} -\frac{55}{6}^{\frac{1}{3}}x^{-3} \\
            y &= \frac{x^3}{6} - 9.167x^{-3} \\
          \end{align*}
      \end{itemize}
  \end{itemize}

  \subsection{9.5.2}
  \begin{itemize}
    \item Solve \(4xy' - 8y = x^{-1}, \qquad y(1) = 6\)
      \[%%%%%%%%%%
      \then y' - 2x^{-1}y = 4x^{-2}
      \]%%%%%%%%%%
      \begin{itemize}
        \item Idetify the integrating factor, \(\alpha(x)\)
          \begin{align*}
            \alpha(x) &= e^{\int -2x^{-1} dx} \\
            \alpha(x) &= e^{-2\ln x} \\
            \alpha(x) &= x^{-2}
          \end{align*}

        \item Find the general solution, \(y(x)\)
          \begin{align*}
            y &= x^{2} \left( \int  x^{-2} 4x^{-2} dx + C \right) \\
            y &= x^{2} \left( -\frac{4}{3}x^{-3}  + C \right) \\
            y &= -\frac{4}{3}x^{-1} + Cx^{2} \\
            \text{?}~&\to\frac{1}{12}x^{-1} + Cx^2
          \end{align*}

        \item Solve the innitla value problem, \(y(1) = 6\)
          \begin{align*}
            6 &= -\frac{1}{12}1^{-1} + C  \\
            C &= 6+\frac{1}{12} = 6.083 \\
            \then
            y &= \frac{1}{12}x^{-1} + 6.083x^2
          \end{align*}
      \end{itemize}
  \end{itemize}

  \subsection{9.5.3}
  \begin{itemize}
    \item Solve \(xy' = 2y - 9x, \qquad y(1) = -2\)
      \[%%%%%%%%%%
      \then y' - 2x^{-1}y = -9
      \]%%%%%%%%%%
      \begin{itemize}
        \item Idetify the integrating factor, \(\alpha(x)\)
          \begin{align*}
            \alpha (x) &= e^{\int -2x^{-1} dx} \\
            \alpha (x) &= e^{-2 \ln  x} \\
            \alpha (x) &= x^{-2}
          \end{align*}

        \item Find the general solution, \(y(x)\)
          \begin{align*}
            y &= x^2 \left( \int -9x^{-2} dx + C\right)  \\
            y &= x^2 (9x^{-1} + C) \\
            y &= 9x + Cx^2
          \end{align*}

        \item Solve the innitla value problem, \(y(1) = -2\)
          \begin{align*}
            -2 &= 9 + C \\
            C &= -11 \\
            \then
            y &= 9x - 11x^2
          \end{align*}
      \end{itemize}
  \end{itemize}

  \subsection{9.5.4}
  \begin{itemize}
    \item Find the general solution of the first-order linear differetial
      equation
      \[%%%%%%%%%%
        y' - (\ln x)y = 2x^{x}
      \]%%%%%%%%%%
      \begin{align*}
        \alpha (x) &= e^{\int -\ln x dx} \\
        \alpha (x) &= e^{x-x\ln x} \\
        \alpha (x) &= e^x x^{-x} \\
        y &= e^{-x}x^x \left( \int e^x x^{-x} 2x^x dx + C \right)  \\
        y &= e^{-x}x^x (2e^x + C) \\
        y &= 2x^x + Ce^{-x}x^{x}
      \end{align*}
  \end{itemize}

  \subsection{9.5.5}
  \begin{itemize}
    \item Solve the initial value problem \(y' + 4y = e^{8x}, \qquad y(0) = -7
      \)
      \begin{align*}
        \alpha (x) &= e^{4x} \\
        y &= e^{-4x} \left( \int e^{4x} 8e^{8x} dx + C \right) \\
        y &= e^{-4x} \left(  \frac{2e^{12x}}{3} + C \right) \\
        y &= \frac{2e^{8x}}{3} + Ce^{-4x} \\
        -7 &= \frac{2}{3} + C \\
        C &= -\frac{23}{3} \\
        y &= \frac{2e^{8x}}{3} - \frac{23e^{-4x}}{3} = \frac{1}{3}(2e^{8x}-23e^{-4x}) \\
          &\text{wrong\ldots} \\
        y &= \frac{e^{8x}}{12} + Ce^{-4x} \\
        -7 &= \frac{1}{12} + C \\
        C &= -\frac{85}{12} \\
        y &= \frac{e^{8x}}{12} + -\frac{85}{12}e^{-4x} \\
      \end{align*}
  \end{itemize}




\end{itemize}
